tests/coq/hashmap/Hashmap_Funs.v
@@ -13,7 +13,7 @@ Definition hash_key_fwd (k : usize) : result usize := Return k.
 
 (** [hashmap::HashMap::{0}::allocate_slots] *)
 Fixpoint hash_map_allocate_slots_loop_fwd
-  (T : Type) (n : nat) (v : vec (List_t T)) (n0 : usize) :
+  (T : Type) (n : nat) (slots : vec (List_t T)) (n0 : usize) :
   result (vec (List_t T))
   :=
   match n with
@@ -21,10 +21,10 @@ Fixpoint hash_map_allocate_slots_loop_fwd
   | S n1 =>
     if n0 s> 0%usize
     then (
-      slots <- vec_push_back (List_t T) v ListNil;
+      slots0 <- vec_push_back (List_t T) slots ListNil;
       n2 <- usize_sub n0 1%usize;
-      hash_map_allocate_slots_loop_fwd T n1 slots n2)
-    else Return v
+      hash_map_allocate_slots_loop_fwd T n1 slots0 n2)
+    else Return slots
   end
 .
 
@@ -57,19 +57,19 @@ Definition hash_map_new_fwd (T : Type) (n : nat) : result (Hash_map_t T) :=
 
 (** [hashmap::HashMap::{0}::clear_slots] *)
 Fixpoint hash_map_clear_slots_loop_fwd_back
-  (T : Type) (n : nat) (v : vec (List_t T)) (i : usize) :
+  (T : Type) (n : nat) (slots : vec (List_t T)) (i : usize) :
   result (vec (List_t T))
   :=
   match n with
   | O => Fail_ OutOfFuel
   | S n0 =>
-    let i0 := vec_len (List_t T) v in
+    let i0 := vec_len (List_t T) slots in
     if i s< i0
     then (
       i1 <- usize_add i 1%usize;
-      slots <- vec_index_mut_back (List_t T) v i ListNil;
-      hash_map_clear_slots_loop_fwd_back T n0 slots i1)
-    else Return v
+      slots0 <- vec_index_mut_back (List_t T) slots i ListNil;
+      hash_map_clear_slots_loop_fwd_back T n0 slots0 i1)
+    else Return slots
   end
 .
 
@@ -176,7 +176,7 @@ Definition core_num_u32_max_c : u32 := core_num_u32_max_body%global.
 
 (** [hashmap::HashMap::{0}::move_elements_from_list] *)
 Fixpoint hash_map_move_elements_from_list_loop_fwd_back
-  (T : Type) (n : nat) (hm : Hash_map_t T) (ls : List_t T) :
+  (T : Type) (n : nat) (ntable : Hash_map_t T) (ls : List_t T) :
   result (Hash_map_t T)
   :=
   match n with
@@ -184,9 +184,9 @@ Fixpoint hash_map_move_elements_from_list_loop_fwd_back
   | S n0 =>
     match ls with
     | ListCons k v tl =>
-      ntable <- hash_map_insert_no_resize_fwd_back T n0 hm k v;
-      hash_map_move_elements_from_list_loop_fwd_back T n0 ntable tl
-    | ListNil => Return hm
+      ntable0 <- hash_map_insert_no_resize_fwd_back T n0 ntable k v;
+      hash_map_move_elements_from_list_loop_fwd_back T n0 ntable0 tl
+    | ListNil => Return ntable
     end
   end
 .
@@ -201,23 +201,24 @@ Definition hash_map_move_elements_from_list_fwd_back
 
 (** [hashmap::HashMap::{0}::move_elements] *)
 Fixpoint hash_map_move_elements_loop_fwd_back
-  (T : Type) (n : nat) (hm : Hash_map_t T) (v : vec (List_t T)) (i : usize) :
+  (T : Type) (n : nat) (ntable : Hash_map_t T) (slots : vec (List_t T))
+  (i : usize) :
   result ((Hash_map_t T) * (vec (List_t T)))
   :=
   match n with
   | O => Fail_ OutOfFuel
   | S n0 =>
-    let i0 := vec_len (List_t T) v in
+    let i0 := vec_len (List_t T) slots in
     if i s< i0
     then (
-      l <- vec_index_mut_fwd (List_t T) v i;
+      l <- vec_index_mut_fwd (List_t T) slots i;
       let ls := mem_replace_fwd (List_t T) l ListNil in
-      ntable <- hash_map_move_elements_from_list_fwd_back T n0 hm ls;
+      ntable0 <- hash_map_move_elements_from_list_fwd_back T n0 ntable ls;
       i1 <- usize_add i 1%usize;
       let l0 := mem_replace_back (List_t T) l ListNil in
-      slots <- vec_index_mut_back (List_t T) v i l0;
-      hash_map_move_elements_loop_fwd_back T n0 ntable slots i1)
-    else Return (hm, v)
+      slots0 <- vec_index_mut_back (List_t T) slots i l0;
+      hash_map_move_elements_loop_fwd_back T n0 ntable0 slots0 i1)
+    else Return (ntable, slots)
   end
 .
 
@@ -267,15 +268,15 @@ Definition hash_map_insert_fwd_back
 
 (** [hashmap::HashMap::{0}::contains_key_in_list] *)
 Fixpoint hash_map_contains_key_in_list_loop_fwd
-  (T : Type) (n : nat) (i : usize) (ls : List_t T) : result bool :=
+  (T : Type) (n : nat) (key : usize) (ls : List_t T) : result bool :=
   match n with
   | O => Fail_ OutOfFuel
   | S n0 =>
     match ls with
     | ListCons ckey t tl =>
-      if ckey s= i
+      if ckey s= key
       then Return true
-      else hash_map_contains_key_in_list_loop_fwd T n0 i tl
+      else hash_map_contains_key_in_list_loop_fwd T n0 key tl
     | ListNil => Return false
     end
   end
@@ -299,15 +300,15 @@ Definition hash_map_contains_key_fwd
 
 (** [hashmap::HashMap::{0}::get_in_list] *)
 Fixpoint hash_map_get_in_list_loop_fwd
-  (T : Type) (n : nat) (i : usize) (ls : List_t T) : result T :=
+  (T : Type) (n : nat) (key : usize) (ls : List_t T) : result T :=
   match n with
   | O => Fail_ OutOfFuel
   | S n0 =>
     match ls with
     | ListCons ckey cvalue tl =>
-      if ckey s= i
+      if ckey s= key
       then Return cvalue
-      else hash_map_get_in_list_loop_fwd T n0 i tl
+      else hash_map_get_in_list_loop_fwd T n0 key tl
     | ListNil => Fail_ Failure
     end
   end
@@ -331,15 +332,15 @@ Definition hash_map_get_fwd
 
 (** [hashmap::HashMap::{0}::get_mut_in_list] *)
 Fixpoint hash_map_get_mut_in_list_loop_fwd
-  (T : Type) (n : nat) (i : usize) (ls : List_t T) : result T :=
+  (T : Type) (n : nat) (key : usize) (ls : List_t T) : result T :=
   match n with
   | O => Fail_ OutOfFuel
   | S n0 =>
     match ls with
     | ListCons ckey cvalue tl =>
-      if ckey s= i
+      if ckey s= key
       then Return cvalue
-      else hash_map_get_mut_in_list_loop_fwd T n0 i tl
+      else hash_map_get_mut_in_list_loop_fwd T n0 key tl
     | ListNil => Fail_ Failure
     end
   end
@@ -353,7 +354,7 @@ Definition hash_map_get_mut_in_list_fwd
 
 (** [hashmap::HashMap::{0}::get_mut_in_list] *)
 Fixpoint hash_map_get_mut_in_list_loop_back
-  (T : Type) (n : nat) (i : usize) (ls : List_t T) (ret : T) :
+  (T : Type) (n : nat) (key : usize) (ls : List_t T) (ret : T) :
   result (List_t T)
   :=
   match n with
@@ -361,10 +362,10 @@ Fixpoint hash_map_get_mut_in_list_loop_back
   | S n0 =>
     match ls with
     | ListCons ckey cvalue tl =>
-      if ckey s= i
+      if ckey s= key
       then Return (ListCons ckey ret tl)
       else (
-        l <- hash_map_get_mut_in_list_loop_back T n0 i tl ret;
+        l <- hash_map_get_mut_in_list_loop_back T n0 key tl ret;
         Return (ListCons ckey cvalue l))
     | ListNil => Fail_ Failure
     end
@@ -406,20 +407,20 @@ Definition hash_map_get_mut_back
 
 (** [hashmap::HashMap::{0}::remove_from_list] *)
 Fixpoint hash_map_remove_from_list_loop_fwd
-  (T : Type) (n : nat) (i : usize) (ls : List_t T) : result (option T) :=
+  (T : Type) (n : nat) (key : usize) (ls : List_t T) : result (option T) :=
   match n with
   | O => Fail_ OutOfFuel
   | S n0 =>
     match ls with
     | ListCons ckey t tl =>
-      if ckey s= i
+      if ckey s= key
       then
         let mv_ls := mem_replace_fwd (List_t T) (ListCons ckey t tl) ListNil in
         match mv_ls with
-        | ListCons i0 cvalue tl0 => Return (Some cvalue)
+        | ListCons i cvalue tl0 => Return (Some cvalue)
         | ListNil => Fail_ Failure
         end
-      else hash_map_remove_from_list_loop_fwd T n0 i tl
+      else hash_map_remove_from_list_loop_fwd T n0 key tl
     | ListNil => Return None
     end
   end
@@ -433,21 +434,21 @@ Definition hash_map_remove_from_list_fwd
 
 (** [hashmap::HashMap::{0}::remove_from_list] *)
 Fixpoint hash_map_remove_from_list_loop_back
-  (T : Type) (n : nat) (i : usize) (ls : List_t T) : result (List_t T) :=
+  (T : Type) (n : nat) (key : usize) (ls : List_t T) : result (List_t T) :=
   match n with
   | O => Fail_ OutOfFuel
   | S n0 =>
     match ls with
     | ListCons ckey t tl =>
-      if ckey s= i
+      if ckey s= key
       then
         let mv_ls := mem_replace_fwd (List_t T) (ListCons ckey t tl) ListNil in
         match mv_ls with
-        | ListCons i0 cvalue tl0 => Return tl0
+        | ListCons i cvalue tl0 => Return tl0
         | ListNil => Fail_ Failure
         end
       else (
-        l <- hash_map_remove_from_list_loop_back T n0 i tl;
+        l <- hash_map_remove_from_list_loop_back T n0 key tl;
         Return (ListCons ckey t l))
     | ListNil => Return ListNil
     end
